src/Arithmetic/MontgomeryReduction/WordByWord/Abstract/Dependent/Definition.v
@@ -25,7 +25,7 @@ Section WordByWordMontgomery.
     {add : forall {n}, T n -> T n -> T (S n)} (* joins carry *)
     {add' : forall {n}, T (S n) -> T n -> T (S (S n))} (* joins carry *)
     {drop_high : T (S (S R_numlimbs)) -> T (S R_numlimbs)} (* drops the highest limb *)
-    {conditional_sub : T (S R_numlimbs) -> T R_numlimbs} (* computes [arg - N] if [R <= arg], and drops high bit *)
+    {conditional_sub : T (S R_numlimbs) -> T R_numlimbs} (* computes [arg - N] if [N <= arg], and drops high bit *)
     (N : T R_numlimbs).
 
   (* Recurse for a as many iterations as A has limbs, varying A := A, S := 0, r, bounds *)
